extraction/theories/TypeAnnotations.v
@@ -561,7 +561,7 @@ Proof.
 Defined.
 
 Definition annot_extract_pcuic_env params Σ wfΣ include ignore :
-  All (annot_transform_type box_type) (transforms params) ->
+  All (annot_transform_type box_type) (extract_transforms params) ->
   match extract_pcuic_env params Σ wfΣ include ignore with
   | Ok Σ => env_annots box_type Σ
   | _ => unit
@@ -577,7 +577,7 @@ Proof.
 Defined.
 
 Definition annot_extract_template_env params Σ include ignore :
-  All (annot_transform_type box_type) (transforms (pcuic_args params)) ->
+  All (annot_transform_type box_type) (extract_transforms (pcuic_args params)) ->
   match extract_template_env params Σ include ignore with
   | Ok Σ => env_annots box_type Σ
   | _ => unit
@@ -585,6 +585,8 @@ Definition annot_extract_template_env params Σ include ignore :
 Proof.
   intros all.
   unfold extract_template_env.
+  destruct (compose_transforms (template_transforms params)); [| exact tt].
+  cbn.
   destruct check_wf_env_func; [|exact tt].
   apply annot_extract_pcuic_env.
   exact all.
